---
title: "Basic Measure Theory and Probability Axioms"
collection: publications
category: probability
permalink: /publication/measuretheory
excerpt: 'We will investigate conditional probability and Bayes theorem.'
date: 2024-09-10
venue: 'Fall'
#slidesurl: 'http://academicpages.github.io/files/slides3.pdf'
#paperurl: 'http://academicpages.github.io/files/paper3.pdf'
citation: 'Jiajun Zhang, (2024) Basic Measure Theory and Probability Axioms'
---


# $\sigma$-Algebra

We begin with some definitions:

**Definition**
Let $\lbrace A_n \rbrace$ be a sequence of sets, the set of all points $\omega \in \Omega$ (where $\Omega$ is the reference set) that belong to $A_n$ for infinitely many values of $n$ is known as the limit supremum of the sequence and is defined by

$$
\lim_{n \rightarrow +\infty} \sup A_n \hspace{0.2cm}
\text{or} \hspace{0.2cm}
\overline{\lim_{n \rightarrow +\infty}} A_n 
$$

Similarly, the set of all points that belong to $A_n$ for all but a finite number of values of $n$ is known as the limit inferior of the sequence $\lbrace A_n \rbrace$ and is denoted by

$$
\lim_{n \rightarrow +\infty} \inf A_n \hspace{0.2cm}
\text{or} \hspace{0.2cm}
\underline{\lim_{n \rightarrow +\infty}} A_n 
$$

If $\displaystyle{\lim_{n \rightarrow +\infty} \sup A_n = \lim_{n \rightarrow +\infty} \inf A_n}$, we say the limit exists and denote $\displaystyle{\lim_{n \rightarrow +\infty}A_n}$ to be its limit.\\


**Corollary**
$$
\underline{\lim_{n \rightarrow +\infty}} A_n = \bigcup_{n=1}^{\infty} \bigcap_{k=n}^{\infty} A_k \subset
\bigcap_{n=1}^{\infty} \bigcup_{k=n}^{\infty} A_k = \overline{\lim_{n \rightarrow +\infty}} A_n
$$


Given the definition of $\lim \sup$ and $\lim \inf$ last lecture, we now give some examples:

1. Let $A_n = \lbrace n \rbrace, n \in \mathbb{N}$, then by definition we have
$$
\underline{\lim_{n \rightarrow \infty}} A_n = \varnothing \hspace{0.5cm} \text{and} \hspace{0.5cm}
\overline{\lim_{n \rightarrow \infty}} A_n = \varnothing
$$

2. Let $A_n = \lbrace (-1)^n \rbrace, n \in \mathbb{N}$, then by definition we have
$$
\underline{\lim_{n \rightarrow \infty}} A_n = \varnothing \hspace{0.5cm} \text{and} \hspace{0.5cm}
\overline{\lim_{n \rightarrow \infty}} A_n = \lbrace -1, 1 \rbrace
$$


**Definition**
1. If $A_n \subset A_{n+1}, n \in \mathbb{N}$, we say $\lbrace A_n \rbrace$ is \textit{non-decreasing}, then $\lim_{n \rightarrow \infty} A_n = \bigcup_{n=1}^{\infty} A_n $.

2. If $A_{n+1} \subset A_n, n \in \mathbb{N}$, we say $\lbrace A_n \rbrace$ is \textit{non-increasing}, then $\lim_{n \rightarrow \infty} A_n = \bigcap_{n=1}^{\infty} A_n$. 


**Definition**
Let $X$ be a space (i.e a non-empty set) and $\mathcal{F}$ be a collection of subsets of $X$ (here $\mathcal{F}$ is the collection of subsets of $X$ which we are going to measure). $\mathcal{F}$ is called a $\sigma$-algebra of subsets of $X$ if:


1. $X \in \mathcal{F}$ 


2. If $A \in \mathcal{F}$, then $A^C := X \backslash A \in \mathcal{F}$. (Closed Under Taking Complement) 


3. If a series of subsets $\lbrace A_n, n \geq 1 \rbrace \in \mathcal{F}$, then $\displaystyle{\bigcup_{n=1}^{\infty}} A_n \in \mathcal{F}$. (Closed Under Countable Union) 


Based on the definition, the following propositions also hold. 


**Corollary**
The definition of $\sigma$-algebra leads to:

\textcircled{1} $\varnothing \in \mathcal{F}$ 

\textcircled{2} $X \in \mathcal{F}$ 

\textcircled{3} If a series of subsets $\lbrace A_n , n \geq 1 \rbrace \in \mathcal{F}$, then $\displaystyle{\bigcap_{n=1}^{\infty} }A_n \in \mathcal{F}$. (Closed Under Countable Intersection)

\textcircled{4} If $A_1, A_2, \cdots, A_N \in \mathcal{F}$, then $\displaystyle{\bigcap_{n=1}^{N} }A_n \in \mathcal{F}$ and $\displaystyle{\bigcup_{n=1}^{N} }A_n \in \mathcal{F}$. (Closed Under Taking Finite Union or Intersection)

\textcircled{5} If $A,B \in \mathcal{F}$, then $A \backslash B, B \backslash A \in \mathcal{F}$


We say $\mathcal{F}_1 $ is bigger than $\mathcal{F}_2$, if $\mathcal{F}_1 \subset \mathcal{F}_2$. In this case, for any space $X$, we may conclude that $\lbrace \varnothing, X \rbrace $ is the smallest $\sigma$-algebra and $2^X$ is the biggest $\sigma$-algebra. A $\sigma$-algebra can also be generated by a collection of sets.

**Definition**
Let $X$ be a space and $\mathcal{C}$ be a collection of subsets of $X$, then the $\sigma$-algebra generated by $\mathcal{C}$, denoted by $\sigma(\mathcal{C})$, is such that

\textcircled{1} $\sigma(\mathcal{C}$) is itself a $\sigma$-algebra with $\mathcal{C}\subset \sigma(\mathcal{C})$

\textcircled{2} If $\mathcal{F}'$ is a $\sigma$-algebra with $\mathcal{C} \subset \mathcal{F}'$, then $\sigma(\mathcal{C}) \subset \mathcal{F}'$. i.e $\sigma(\mathcal{C})$ is the smallest $\sigma$-algebra that is a super set of $\mathcal{C}$. 



Again, we have the following propositions:


**Corollary**


\textcircled{1} $\sigma(\mathcal{C}) = \displaystyle{\bigcap} \left\{ \mathcal{F} : \mathcal{C} \subset \mathcal{F} \right\}$ for all $\sigma$-algebra $\mathcal{F}$

\textcircled{2} If $\mathcal{C}$ itself is a $\sigma$-algebra, then $\sigma(\mathcal{C}) = \mathcal{C}$

\textcircled{3} If $\mathcal{C}_1, \mathcal{C}_2$ are 2 collections of subsets of $X$ with $\mathcal{C}_1 \subset \mathcal{C}_2$, then $\sigma(\mathcal{C}_1) \subset \sigma(\mathcal{C}_2) $




# Borel $\sigma$-Algebra

An important example of $\sigma$-algebra on  $\mathbb{R}$ (of subsets of $\mathbb{R})$ is called a Borel $\sigma$-Algebra.

**Definition**
The Borel $\sigma$-algebra of $\mathbb{R}$ is defined by
$$
\mathfrak{B}_{\mathbb{R}} := \sigma( \lbrace \text{Open Sets of $\mathbb{R}$} \rbrace )
$$



Also we need to know that the generator of $\mathfrak{B}{\mathbb{R}}$ is not unique. By standard definition, we give

$$
\mathfrak{B}_{\mathbb{R}} := \sigma( \lbrace (a,b) : a,b \in \mathbb{R}, a < b \rbrace )
$$

But we still have the following proposition: 

**Corollary**
$$
\begin{align*}
&\textcircled{1} \mathfrak{B}_{\mathbb{R}} := \sigma( \lbrace (a,b] : a,b \in \mathbb{R}, a < b \rbrace )\\
&\textcircled{2} \mathfrak{B}_{\mathbb{R}} := \sigma( \lbrace [a,b) : a,b \in \mathbb{R}, a < b \rbrace )\\
&\textcircled{3} \mathfrak{B}_{\mathbb{R}} := \sigma( \lbrace [a,b] : a,b \in \mathbb{R}, a < b \rbrace )\\
&\textcircled{4} \mathfrak{B}_{\mathbb{R}} := \sigma( \lbrace (-\infty,c) : c \in \mathbb{Q} )\\
&\textcircled{5} \mathfrak{B}_{\mathbb{R}} := \sigma( \lbrace (c,+\infty) : c \in \mathbb{Q} )
\end{align*}
$$

I shall illustrate why those are indeed equal. Let's just take a look at \textcircled{2}, we need to show

$$
\sigma( \lbrace (a,b) : a,b \in \mathbb{R}, a < b \rbrace ) = \sigma( \lbrace [a,b) : a,b \in \mathbb{R}, a < b \rbrace )
$$

We could indeed prove $L.H.S \subset R.H.S$ and $R.H.S \subset L.H.S$.

$\bullet$ To show that $L.H.S \subset R.H.S$, we need to show

$$
(a,b) \in \sigma( \lbrace [a,b) : a,b \in \mathbb{R}, a < b \rbrace )
$$

and we have

$$
(a,b) = \bigcup_{n=1}^{\infty} \left[a + \frac{1}{n} , b \right) \in R.H.S
$$

$\bullet$ Similarly,

$$
[a,b) = \bigcap_{n=1}^{\infty} \left(a - \frac{1}{n} , b \right) \in L.H.S
$$

And that's why they are indeed equal. 

**Definition**
A set $G$ is called a Borel Set if $G \in \mathfrak{B}_{\mathbb{R}}$.

In fact, any set produced by countable operations are also Borel Sets.


**Corollary**
A set with a single element (or singletons) $\lbrace x \rbrace$ is also a Borel Set.


**Proof**
For a singleton $x \in \mathbb{R}$, we have

$$
\lbrace x \rbrace = \bigcap_{n=1}^{\infty} \left( x - \frac{1}{n} , x+ \frac{1}{n} \right).
$$
**QED**



\newpage

\newpage
\section{Measures}

Given a space $X$ and a $\sigma$-algebra $\mathcal{F}$ of subsets of $X$, $(X,\mathcal{F})$ is called a measurable space.

**Definition**
Given a measure space $(X,\mathcal{F})$, define

$$
\mu : \mathcal{F} \longrightarrow [0,+\infty]
$$
is a non-negative set function, then $\mu$ is a measure if

\textcircled{1} $\mu \lbrace \varnothing \rbrace = 0$;

\textcircled{2} If $\lbrace A_n, n \geq 1 \rbrace \subset \mathcal{F}$ such that $A_n$'s are (pairwise) disjoint, then

$$
\mu \left\{ \bigcup_{n=1}^{\infty} A_n \right\} = 
\sum_{n=1}^{\infty} \mu (A_n)
$$

this is known as countable additivity.



We say that $\mu$ is finite if $\mu(X) < +\infty$, we say that $\mu$ is a \textit{probability measure} if $\mu(X) = 1$.

We say $\mu$ is \textit{$\sigma$-finite} if $\exists \lbrace A_n , n \geq 1\rbrace \subset \mathcal{F}$ such that $\displaystyle{X = \bigcup_{n=1}^{\infty} A_n}$ with $\mu(A_n) < +\infty$.

\begin{center}
We call the triple $(X,\mathcal{F},\mu)$ a measure space.
\end{center}

Here are a few examples of measures on $(\mathbb{R},\mathfrak{B}_{\mathbb{R}})$:

\textcircled{1} A measure $\mu_1$ given by

$$
\mu_1 : \mathfrak{B}_{\mathbb{R}} \longrightarrow [0,+\infty], \text{such that} \hspace{0.2cm} \forall A \in \mathfrak{B}_{\mathbb{R}},
\mu_1(A) = \begin{cases} \vert A \vert, \text{if $A$ is finite} \\ \\+\infty, \text{otherwise} \end{cases}
$$

We say $\mu_1$ is the counting measure.

\textcircled{2} Let $x_0 \in \mathbb{R}$, a measure $\mu_2$ is such that
$$
\forall A \in \mathfrak{B}_{\mathbb{R}}, \mu_2(A) = 
\begin{cases} 1, (x_0 \in A) \\ \\ 0, (x_0 \notin A) 
\end{cases}
$$

We say $\mu_2$ is the probability measure.




We now give some propositions for the measure space. Below, let $(X,\mathcal{F}, \mu)$ be a measure space.

**Corollary**
 (Finite Additivity)

If $A_1,A_2,\cdots,A_N \in \mathcal{F}$ are disjoint, then
$$
\mu\left(A_1 \bigcup A_2 \bigcup \cdots \bigcup A_N \right) = \sum_{n=1}^N \mu(A_n).
$$


**Corollary**
(Monotoncity)

Given $A,B \in \mathcal{F}$, if $A \subset B$, then $\mu(A) \leq \mu(B)$.


**Proof**
Note that since $\mu(A),\mu(B)$ could both be infinite, so taking $\mu(B)-\mu(A)$ is incorrect. Indeed, we may construct $B = A \bigcup (B \backslash A)$, where
$$
\mu(B) = \mu(A) + \mu(B \backslash A) \geq \mu(A).
$$
**QED**

**Corollary**
(Countable / Finite Subadditivity)

If $\lbrace A_n, n \geq 1 \rbrace \subset \mathcal{F}$, then
$$
\mu \left( \bigcup_{n=1}^{\infty} A_n \right) \leq 
\sum_{n=1}^{\infty} \mu(A_n) \hspace{0.2cm} \text{and} \hspace{0.2cm} 
\mu \left( \bigcup_{n=1}^{N} A_n \right) \leq 
\sum_{n=1}^{N} \mu(A_n) 
$$
Note that if $A_n$'s are disjoint, then it should be "$=$". 


**Proof**
Let $B_1 = A_1$, and $B_n := A_n \backslash \left( \bigcup_{i=1}^{n-1} A_i \right)$ for every $n \geq 2$, then we know that $\lbrace B_n, n \geq 1 \rbrace \subset \mathcal{F}$ and $B_n$'s are disjoint. More importantly, by our construction we have $\bigcup_{n=1}^{\infty} B_n = \bigcup_{n=1}^{\infty} A_n$. Thus by countable additivity, we have
$$
\mu \left( \bigcup_{n=1}^{\infty} A_n \right) = \mu \left( \bigcup_{n=1}^{\infty} B_n \right) = \sum_{n=1}^{\infty} \mu(B_n) \leq \sum_{n=1}^{\infty} \mu(A_n)
$$
**QED**

**Corollary**
 (Coutinuity From Below)

Given $\lbrace A_n , n\geq 1\rbrace \subset \mathcal{F}$ such that $A_n \subset A_{n+1}$ for every $n$, then
$$
\mu\left(\bigcup_{n=1}^{\infty} A_n \right) = \lim_{n \rightarrow \infty} \mu(A_n)
$$

**Proof**
Set $B_1 = A_1$, $B_n = A_n \backslash A_{n-1}$ for all $n \geq 2$. By definition we have $\lbrace B_n, n \geq 1 \rbrace \subset \mathcal{F}$ is disjoint, and we have
$\bigcup_{n=1}^{\infty} B_n = \bigcup_{n=1}^{\infty} A_n$; also for each $N \geq 1$, $\bigcup_{n=1}^N B_n = A_n$, which means
$$
\begin{align*}
\mu \left( \bigcup_{n=1}^{\infty} A_n \right) = 
\mu \left( \bigcup_{n=1}^{\infty} B_n \right) = 
\sum_{n=1}^{\infty} \mu(B_n) &= \lim_{N \rightarrow \infty} \sum_{n=1}^{N} \mu(B_n)\\
&= \lim_{N \rightarrow \infty} \mu \left( \bigcup_{n=1}^N B_n \right)\\
&= \lim_{n \rightarrow \infty} (A_n)
\end{align*}
$$
**QED**

**Corollary**
 (Continuity From Above)

Given $\lbrace A_n, n \geq 1 \rbrace \in \mathcal{F}$ such that $A_{n+1} \subset A_n$ for every $n \geq 1$, if $\mu(A_1) < +\infty$, then

$$
\mu \left( \bigcap_{n=1}^{\infty} A_n \right) = 
\lim_{n \rightarrow \infty} \mu(A_n)
$$


**Proof**
Set $B_n = A_1 \backslash A_n$, then we know that the sequence $\lbrace B_n , n\geq 1 \rbrace$ is increasing, then we have

$$
\bigcup_{n=1}^{\infty} B_n = A_1 \backslash \bigcap_{n=1}^{\infty} A_n
$$
Thus,

$$
\mu \left( A_1 \backslash \bigcap_{n=1}^{\infty} A_n \right)= \mu \left( \bigcup_{n=1}^{\infty} B_n \right)
= \lim_{n \rightarrow \infty} \mu(B_n) = \lim_{n \rightarrow \infty} \mu(A \backslash A_n) \hspace{3cm} (*)
$$

Given that the measure of $A_n$ is always finite, so
$\mu(A_1 \backslash A_n ) = \mu(A_1) - \mu(A_n)$ and

$$
\mu \left( A_1 \backslash \bigcap_{n=1}^{\infty} A_n \right)= \mu(A_1) - \mu \left( \bigcap_{n=1}^{\infty} A_n \right)
$$

Thus, by equation $(*)$, 

$$
\mu(A_1) - \mu \left( \bigcap_{n=1}^{\infty} A_n \right)
= \lim_{n \rightarrow \infty} \left(\mu(A_1) - \mu(A_n)\right)
$$
that is

$$
\mu \left( \bigcap_{n=1}^{\infty} A_n \right) = 
\lim_{n \rightarrow \infty} \mu(A_n)
$$
**QED**


The reason why we would introduce the definition of a $\sigma$-algebra, measure is that, probability, is also a measure. 



# An introduction to sample spaces and probability axioms

**Definition**
A random (or a statistical) experiment is an experiment with the following:

\textcircled{1} All outcomes of the experiment are known in advance;

\textcircled{2} Any performance of the experiment results in an outcome is not known i advance;

\textcircled{3} The experiment can be repeated under identical conditions.


**Definition**
The sample space of a statistical experiment is a pair $(\Omega, \mathcal{F})$ where $\Omega$ is the set of all possible outcomes of the experiment and $\mathcal{F}$ is a $\sigma$ field of the subsets of $\Omega$.



Here is an example to illustrate this: Suppose we are tossing a coin, and we denote $H$ (head) and $T$ (tail) to be the only two possible outcomes. Then we have $\Omega := \lbrace H,T \rbrace$ and $\mathcal{F} := \lbrace \{ H \} , \{ T \}, \{ H,T \} , \varnothing \rbrace$. Element of $\Omega$ are called the \textit{sample points} and any set $A \in \mathcal{F}$ is called an event.

**Definition**
(Kolmogorov's Axioms)


Let $(\Omega,\mathcal{F})$ be a sample space and a set function $\P : \mathcal{F} \longrightarrow \mathbb{R}$ is called a probability measure (or simply probability) if it satisfies:\\

\textcircled{1} $\P(A) \geq 0$ for all $A \in \mathcal{F}$;\\

\textcircled{2} $\P(\Omega) = 1$;\\

\textcircled{3} Let $\{ A_j \}_1^{\infty}$ be a sequence of disjoint sets where $A_j \in \mathcal{F}$, then $\displaystyle{\P \left( \bigcup_{i=1}^{\infty} A_i \right) = \sum_{i =1}^{\infty} \P(A_i)}$.



**Corollary**
$\P$ is monotone and substrative, i.e if $A,B \in \mathcal{F}$ with $A \subset B$, then $\P(A) \leq \P(B)$.


**Corollary**
If $A \in \mathcal{F}$, then $\P(A) = 1 - \P(A^C)$.


Now we will introduce an important theorem in probability:

**Theorem**
(The principle of inclusion and exclusion)

Let $A_1,A_2,\cdots,A_n \in \mathcal{F}$, then

$$
\P \left( \bigcup_{k=1}^n A_k \right) = \sum_{k=1}^{n} \P(A_k) - \sum_{k_1<k_2}\P(A_{k_1} \cap A_{k_2}) + \cdots + (-1)^{n+1} \sum_{k_1<\cdots<k_n} \P(A_{k_1} \cap \cdots \cap  A_{k_n})
$$


**Proof**
 We will first consider some special cases, let's say $n=2$, then we have
$$
\P(A_1 \cup A_2) = \P(A_1) + \P(A_2) - \P(A_1 \cap A_2).
$$

Similarly, consider $n=3$, then we have
$$
\begin{align*}
\P(A_1 \cup A_2 \cup A_3) &= \P(A_1) + \P(A_2) + \P(A_3)\\
& -\P(A_1 \cap A_2) - \P(A_2 \cap A_3) - \P(A_1 \cap A_3) \\
& + \P(A_1 \cap A_2 \cap A_3)
\end{align*}
$$

So when $n=2$ or $n=3$, it is already proven according to the construction we did using Venn diagram. Now we perform the induction on $n$, assume it holds for some number $N (N>3)$, then say
$$
\P \left( \bigcup_{i=1}^{N+1} A_i \right) = \P \left( \left[ \bigcup_{i=1}^N A_i \right] \bigcup A_{N+1} \right)
$$
Denote $\left[ \bigcup_{i=1}^N A_i \right] = B$, then we have
$$
\P \left( \bigcup_{i=1}^{N+1} A_i \right) = \P(B) + \P(A_{N+1}) - \P(B \cap A_{N+1})
$$
**QED**


The principle of inclusion and exculsion also leads us to another theorem:

**Theorem**
(Bonferroni's Inequality)

Given $n$ events $A_1,A_2,\cdots,A_n \in \mathcal{F}, (n>1)$, then 
$$
\sum_{k=1}^n \P(A_k) - \sum_{i<j} \P(A_i \cap A_j) \leq \P \left( \sum_{k=1}^n A_k \right) \leq \sum_{k=1}^n \P(A_k)
$$


**Proof**
The proof is basically the same idea as above, reader should try to prove this by their own.
**QED**

**Theorem**
(Boole's Inequality)

Suppose $A,B \in \mathcal{F}$, then
$$
\P(A \cap B) \geq 1 - \P(A^C) - \P(B^C)
$$


**Proof**
$$
\begin{align*}
\P(A \cap B) &= 1 - \P((A \cap B)^C) \\
&= 1 - \P(A^C \cup B^C)\\
&= 1 - (\P(A^C) + \P(B^C) - \P(A^C \cap B^C))\\
&\geq 1 - \P(A^C) - \P(B^C)
\end{align*}
$$
**QED**


**Corollary**
Let $\{ A_j \}_{j=1}^{\infty}$ be a sequence of events, then 
$$
\P \left(\bigcap_{j=1}^{\infty} A_j \right) \geq 1 - \sum_{j=1}^{\infty} \P(A_j^C)
$$


**Proof**
This proof can be achieved by induction, using the results in theorem 4.
**QED**


**Theorem**
(The implicative rule)

If $A_1,A_2,A_3 \in \mathcal{F}$ and $A_1 \cap A_2 \subset A_3$, i.e $A_1,A_2$ implies $A_3$, then $\P(A_3^C) \leq \P(A_1^C) + \P(A_2^C)$.



**Proof**
By monotoncity of probability, we have $\P(A_1 \cap A_2) \leq \P(A_3)$, i.e $\P((A_1 \cap A_2)^C) \geq \P(A_3^C)$, that is $\P(A_1^C \cap A_2^C) \geq \P(A_3^C)$, by inclusion and exculsion formula, we have $\P(A_1^C) + \P(A_2^C) - P(A_1^C \cap A_2^C) \geq \P(A_3^C)$, given that the probability is always non-negative, we then conclude that $\P(A_3^C) \leq \P(A_1^C) + \P(A_2^C)$.
**QED**

**Theorem**
(Continuity of $\P$)

Let $\{ A_n \}_{n=1}^{\infty}$ be a sequence of non-decreasing events in $\mathcal{F}$, i.e $A_n \subset A_{n+1}$, then
$$
\P(\lim_{n \to \infty} A_n) = \lim_{n \to \infty} \P(A_n) = \P \left( \bigcup_{n=1}^{\infty} A_n \right)
$$


**Proof**
Let $A = \bigcup_{j=1}^{\infty} A_j$, then $A$ can be written as $A = A_n \bigcup \left( \bigcup_{j=n}^{\infty} A_{j+1} \backslash A_j \right)$, by $\sigma$ additivity, we also have 

$$
\begin{align*}
\P(A) &= \P(A_n) + \sum_{j=n}^{\infty} \P(A_{j+1} \backslash A_j) \\
& = \P(A_n) + \sum_{j=n}^{\infty}  \left( \P(A_{j+1}) - \P(A_j) \right)
\end{align*}
$$
Now taking $n \to \infty$:

$$
\begin{align*}
\P(A) &= \lim_{n \to \infty} \left[ \P(A_n) + \sum_{j=n}^{\infty} (\P(A_{j+1}) - P(A_j) ) \right] \\
&= \lim_{n \to \infty} A_n + \lim_{n \to \infty} \left[ \sum_{j=n}^{\infty} \P(A_{j+1}) - \P(A_j) \right]\\
&= \lim_{n \to \infty} \P(A_n)
\end{align*}
$$
**QED**

**Theorem**
(Continuity of $\P$)

Let $\{ A_n \}_{n=1}^{\infty}$ be a sequence of non-increasing events in $\mathcal{F}$, i.e $A_{n+1} \subset A_n$, then
$$
\P(\lim_{n \to \infty} A_n) = \lim_{n \to \infty} \P(A_n) = \P \left( \bigcap_{n=1}^{\infty} A_n \right)
$$


**Proof**
This can be done by taking $B_n = A_n^C$.
**QED**
